fix most of otbn arch

arch/otbn/interp.i.dfy
@@ -1,67 +1,34 @@
-include "vt_consts.dfy"
-include "bv_ops.dfy"
+include "machine.s.dfy"
 
-module vt_mem {
+module ot_interp {
     import opened bv_ops
-    import opened vt_consts
+    import opened ot_machine
 
-/* mem_t definion */
+/* wdr_view definion (SHADOW) */
 
-    // admissible is aligned and bounded
-    predicate method xword_ptr_admissible(ptr: nat)
+    datatype uint512_raw = uint512_cons(
+        lh: uint256, uh: uint256, full: uint512)
+
+    type uint512_view_t = num: uint512_raw |
+        && num.lh == uint512_lh(num.full)
+        && num.uh == uint512_uh(num.full)
+        witness *
+
+    predicate valid_uint512_view(
+        wdrs: wdrs_t, num: uint512_view_t,
+        li: int, ui: int)
+        requires -1 <= li < BASE_5;
+        requires -1 <= ui < BASE_5;
     {
-        && ptr % 4 == 0
-        && ptr < DMEM_LIMIT
+        && (li == NA || wdrs[li] == num.lh)
+        && (ui == NA || wdrs[ui] == num.uh)
     }
 
-    // admissible is aligned and bounded
-    predicate method wword_ptr_admissible(ptr: nat)
-    {
-        && ptr % 32 == 0
-        && ptr < DMEM_LIMIT
-    }
-
-    type mem_t = map<int, uint32>
-
-    predicate method wword_ptr_valid(mem: mem_t, ptr: nat)
-    {
-        && wword_ptr_admissible(ptr)
-        && ptr + 0 in mem
-        && ptr + 4 in mem
-        && ptr + 8 in mem
-        && ptr + 12 in mem
-        && ptr + 16 in mem
-        && ptr + 20 in mem
-        && ptr + 24 in mem
-        && ptr + 28 in mem
-    }
-
-    function method read_wword(mem: mem_t, ptr: nat): uint256
-        requires wword_ptr_valid(mem, ptr)
-    {
-        var p0 := mem[ptr + 0];
-        var p1 := mem[ptr + 4];
-        var p2 := mem[ptr + 8];
-        var p3 := mem[ptr + 12];
-        var p4 := mem[ptr + 16];
-        var p5 := mem[ptr + 20];
-        var p6 := mem[ptr + 24];
-        var p7 := mem[ptr + 28];
-        uint256_eighth_assemble(p0, p1, p2, p3, p4, p5, p6, p7)
-    }
-
-    function method mem_write_wword(mem: mem_t, ptr: nat, value: uint256): (mem' : mem_t)
-        requires wword_ptr_admissible(ptr)
-        ensures wword_ptr_valid(mem', ptr)
-    {
-        mem[ptr + 0 := uint256_eighth_split(value, 0)]
-            [ptr + 4 := uint256_eighth_split(value, 1)]
-            [ptr + 8 := uint256_eighth_split(value, 2)]
-            [ptr + 12 := uint256_eighth_split(value, 3)]
-            [ptr + 16 := uint256_eighth_split(value, 4)]
-            [ptr + 20 := uint256_eighth_split(value, 5)]
-            [ptr + 24 := uint256_eighth_split(value, 6)]
-            [ptr + 28 := uint256_eighth_split(value, 7)]
+    predicate valid_wdr_view(wdrs: wdrs_t, view: seq<uint256>, start: nat, len: nat)
+    {   
+        && |view| == len
+        && start + len <= 32
+        && wdrs[start..start+len] == view
     }
 
 /* heap_t definion (SHADOW) */
